kkk

examples/n_german/ABS_german_1.thy
@@ -1,167 +1,65 @@
 theory ABS_german_1
-  imports Symmetric
+  imports CMP
 begin
-section{*Main definitions*}
-definition I::"scalrValueType" where [simp]: "I\<equiv> enum ''control'' ''I''"
-definition S::"scalrValueType" where [simp]: "S\<equiv> enum ''control'' ''S''"
-definition E::"scalrValueType" where [simp]: "E\<equiv> enum ''control'' ''E''"
-definition Empty::"scalrValueType" where [simp]: "Empty\<equiv> enum ''control'' ''Empty''"
-definition ReqS::"scalrValueType" where [simp]: "ReqS\<equiv> enum ''control'' ''ReqS''"
-definition ReqE::"scalrValueType" where [simp]: "ReqE\<equiv> enum ''control'' ''ReqE''"
-definition Inv::"scalrValueType" where [simp]: "Inv\<equiv> enum ''control'' ''Inv''"
-definition InvAck::"scalrValueType" where [simp]: "InvAck\<equiv> enum ''control'' ''InvAck''"
-definition GntS::"scalrValueType" where [simp]: "GntS\<equiv> enum ''control'' ''GntS''"
-definition GntE::"scalrValueType" where [simp]: "GntE\<equiv> enum ''control'' ''GntE''"
+
+subsection \<open>Definitions\<close>
+
+text \<open>type definitions \<close>
+
+definition I :: scalrValueType where [simp]: "I\<equiv> enum ''control'' ''I''"
+definition S :: scalrValueType where [simp]: "S\<equiv> enum ''control'' ''S''"
+definition E :: scalrValueType where [simp]: "E\<equiv> enum ''control'' ''E''"
+definition Empty :: scalrValueType where [simp]: "Empty\<equiv> enum ''control'' ''Empty''"
+definition ReqS :: scalrValueType where [simp]: "ReqS\<equiv> enum ''control'' ''ReqS''"
+definition ReqE :: scalrValueType where [simp]: "ReqE\<equiv> enum ''control'' ''ReqE''"
+definition Inv :: scalrValueType where [simp]: "Inv\<equiv> enum ''control'' ''Inv''"
+definition InvAck :: scalrValueType where [simp]: "InvAck\<equiv> enum ''control'' ''InvAck''"
+definition GntS :: scalrValueType where [simp]: "GntS\<equiv> enum ''control'' ''GntS''"
+definition GntE :: scalrValueType where [simp]: "GntE\<equiv> enum ''control'' ''GntE''"
 definition true::"scalrValueType" where [simp]: "true\<equiv> boolV True"
 definition false::"scalrValueType" where [simp]: "false\<equiv> boolV False"
 
-definition n_RecvGntE1::"nat \<Rightarrow> rule" where [simp]:
-"n_RecvGntE1  i\<equiv>
-let g = (eqn (IVar (Para (''Chan2.Cmd'') i)) (Const GntE)) in
-let s = (parallelList [(assign (Para (''Cache.State'') i, (Const E))), (assign (Para (''Cache.Data'') i, (IVar (Para (''Chan2.Data'') i)))), (assign (Para (''Chan2.Cmd'') i, (Const Empty)))]) in
-guard g s"
-
-definition n_RecvGntS2::"nat \<Rightarrow> rule" where [simp]:
-"n_RecvGntS2  i\<equiv>
-let g = (eqn (IVar (Para (''Chan2.Cmd'') i)) (Const GntS)) in
-let s = (parallelList [(assign (Para (''Cache.State'') i, (Const S))), (assign (Para (''Cache.Data'') i, (IVar (Para (''Chan2.Data'') i)))), (assign (Para (''Chan2.Cmd'') i, (Const Empty)))]) in
-guard g s"
-
-definition n_SendGntE3::"nat \<Rightarrow> nat \<Rightarrow> rule" where [simp]:
-"n_SendGntE3  i N\<equiv>
-let g = (andList [(eqn (IVar (Ident ''CurCmd'')) (Const ReqE)) , (eqn (IVar (Ident ''CurPtr'')) (Const (index i))) , (eqn (IVar (Para (''Chan2.Cmd'') i)) (Const Empty)) , (eqn (IVar (Ident ''ExGntd'')) (Const false)) , (forallForm (down N) (\<lambda>j. (eqn (IVar (Para (''ShrSet'') j)) (Const false)) ))])in
-let s = (parallelList [(assign (Para (''Chan2.Cmd'') i, (Const GntE))), (assign (Para (''Chan2.Data'') i, (IVar (Ident ''MemData'')))), (assign (Para (''ShrSet'') i, (Const true))), (assign ((Ident ''ExGntd''), (Const true))), (assign ((Ident ''CurCmd''), (Const Empty)))]) in
-guard g s"
-
-definition n_SendGntS4::"nat \<Rightarrow> rule" where [simp]:
-"n_SendGntS4  i\<equiv>
-let g = (andList [(eqn (IVar (Ident ''CurCmd'')) (Const ReqS)) , (eqn (IVar (Ident ''CurPtr'')) (Const (index i))) , (eqn (IVar (Para (''Chan2.Cmd'') i)) (Const Empty)) , (eqn (IVar (Ident ''ExGntd'')) (Const false)) ])in
-let s = (parallelList [(assign (Para (''Chan2.Cmd'') i, (Const GntS))), (assign (Para (''Chan2.Data'') i, (IVar (Ident ''MemData'')))), (assign (Para (''ShrSet'') i, (Const true))), (assign ((Ident ''CurCmd''), (Const Empty)))]) in
-guard g s"
-
-definition n_RecvInvAck5::"nat \<Rightarrow> rule" where [simp]:
-"n_RecvInvAck5  i\<equiv>
-let g = (andList [(eqn (IVar (Para (''Chan3.Cmd'') i)) (Const InvAck)) , (eqn (IVar (Ident ''CurCmd !'')) (Const Empty)) , (eqn (IVar (Ident ''ExGntd'')) (Const true)) ])in
-let s = (parallelList [(assign (Para (''Chan3.Cmd'') i, (Const Empty))), (assign (Para (''ShrSet'') i, (Const false))), (assign ((Ident ''ExGntd''), (Const false))), (assign ((Ident ''MemData''), (IVar (Para (''Chan3.Data'') i))))]) in
-guard g s"
-
-definition n_RecvInvAck6::"nat \<Rightarrow> rule" where [simp]:
-"n_RecvInvAck6  i\<equiv>
-let g = (andList [(eqn (IVar (Para (''Chan3.Cmd'') i)) (Const InvAck)) , (eqn (IVar (Ident ''CurCmd !'')) (Const Empty)) , (eqn (IVar (Ident ''ExGntd !'')) (Const true)) ])in
-let s = (parallelList [(assign (Para (''Chan3.Cmd'') i, (Const Empty))), (assign (Para (''ShrSet'') i, (Const false)))]) in
-guard g s"
-
-definition n_SendInvAck7::"nat \<Rightarrow> rule" where [simp]:
-"n_SendInvAck7  i\<equiv>
-let g = (andList [(eqn (IVar (Para (''Chan2.Cmd'') i)) (Const Inv)) , (eqn (IVar (Para (''Chan3.Cmd'') i)) (Const Empty)) , (eqn (IVar (Para (''Cache.State'') i)) (Const E)) ])in
-let s = (parallelList [(assign (Para (''Chan2.Cmd'') i, (Const Empty))), (assign (Para (''Chan3.Cmd'') i, (Const InvAck))), (assign (Para (''Chan3.Data'') i, (IVar (Para (''Cache.Data'') i)))), (assign (Para (''Cache.State'') i, (Const I)))]) in
-guard g s"
-
-definition n_SendInvAck8::"nat \<Rightarrow> rule" where [simp]:
-"n_SendInvAck8  i\<equiv>
-let g = (andList [(eqn (IVar (Para (''Chan2.Cmd'') i)) (Const Inv)) , (eqn (IVar (Para (''Chan3.Cmd'') i)) (Const Empty)) , (eqn (IVar (Para (''Cache.State !'') i)) (Const E)) ])in
-let s = (parallelList [(assign (Para (''Chan2.Cmd'') i, (Const Empty))), (assign (Para (''Chan3.Cmd'') i, (Const InvAck))), (assign (Para (''Cache.State'') i, (Const I)))]) in
-guard g s"
-
-definition n_SendInv9::"nat \<Rightarrow> rule" where [simp]:
-"n_SendInv9  i\<equiv>
-let g = (andList [(eqn (IVar (Para (''Chan2.Cmd'') i)) (Const Empty)) , (eqn (IVar (Para (''InvSet'') i)) (Const true)) , (eqn (IVar (Ident ''CurCmd'')) (Const ReqE)) ])in
-let s = (parallelList [(assign (Para (''Chan2.Cmd'') i, (Const Inv))), (assign (Para (''InvSet'') i, (Const false)))]) in
-guard g s"
-
-definition n_SendInv10::"nat \<Rightarrow> rule" where [simp]:
-"n_SendInv10  i\<equiv>
-let g = (andList [(eqn (IVar (Para (''Chan2.Cmd'') i)) (Const Empty)) , (eqn (IVar (Para (''InvSet'') i)) (Const true)) , (eqn (IVar (Ident ''CurCmd'')) (Const ReqS)) , (eqn (IVar (Ident ''ExGntd'')) (Const true)) ])in
-let s = (parallelList [(assign (Para (''Chan2.Cmd'') i, (Const Inv))), (assign (Para (''InvSet'') i, (Const false)))]) in
-guard g s"
-
-definition n_RecvReqE11::"nat \<Rightarrow> nat \<Rightarrow> rule" where [simp]:
-"n_RecvReqE11  i N\<equiv>
-let g = (andList [(eqn (IVar (Ident ''CurCmd'')) (Const Empty)) , (eqn (IVar (Para (''Chan1.Cmd'') i)) (Const ReqE)) ])in
-let s = (parallelList [(assign ((Ident ''CurCmd''), (Const ReqE))), (assign ((Ident ''CurPtr''), (Const (index i)))), (assign (Para (''Chan1.Cmd'') i, (Const Empty))), (parallelList (map (\<lambda>j. (assign (Para (''InvSet'') j, (IVar (Para (''ShrSet'') j))))) (down N)))]) in
-guard g s"
-
-definition n_RecvReqS12::"nat \<Rightarrow> nat \<Rightarrow> rule" where [simp]:
-"n_RecvReqS12  i N\<equiv>
-let g = (andList [(eqn (IVar (Ident ''CurCmd'')) (Const Empty)) , (eqn (IVar (Para (''Chan1.Cmd'') i)) (Const ReqS)) ])in
-let s = (parallelList [(assign ((Ident ''CurCmd''), (Const ReqS))), (assign ((Ident ''CurPtr''), (Const (index i)))), (assign (Para (''Chan1.Cmd'') i, (Const Empty))), (parallelList (map (\<lambda>j. (assign (Para (''InvSet'') j, (IVar (Para (''ShrSet'') j))))) (down N)))]) in
-guard g s"
-
-definition n_SendReqE13::"nat \<Rightarrow> rule" where [simp]:
-"n_SendReqE13  i\<equiv>
-let g = (andList [(eqn (IVar (Para (''Chan1.Cmd'') i)) (Const Empty)) , (eqn (IVar (Para (''Cache.State'') i)) (Const I)) ])in
-let s = (parallelList [(assign (Para (''Chan1.Cmd'') i, (Const ReqE)))]) in
-guard g s"
-
-definition n_SendReqE14::"nat \<Rightarrow> rule" where [simp]:
-"n_SendReqE14  i\<equiv>
-let g = (andList [(eqn (IVar (Para (''Chan1.Cmd'') i)) (Const Empty)) , (eqn (IVar (Para (''Cache.State'') i)) (Const S)) ])in
-let s = (parallelList [(assign (Para (''Chan1.Cmd'') i, (Const ReqE)))]) in
-guard g s"
-
-definition n_SendReqS15::"nat \<Rightarrow> rule" where [simp]:
-"n_SendReqS15  i\<equiv>
-let g = (andList [(eqn (IVar (Para (''Chan1.Cmd'') i)) (Const Empty)) , (eqn (IVar (Para (''Cache.State'') i)) (Const I)) ])in
-let s = (parallelList [(assign (Para (''Chan1.Cmd'') i, (Const ReqS)))]) in
-guard g s"
-
-definition n_Store16::"nat \<Rightarrow> rule" where [simp]:
-"n_Store16  i\<equiv>
-let g = (eqn (IVar (Para (''Cache.State'') i)) (Const E)) in
-let s = (parallelList [(assign (Para (''Cache.Data'') i, (IVar(Ident ''d'')))), (assign ((Ident ''AuxData''), (IVar(Ident ''d''))))]) in
-guard g s"
-
-definition rules::"nat \<Rightarrow> rule set" where [simp]:
-"rules N \<equiv> {r.
-(\<exists> i. i\<le>N\<and>r=n_RecvGntE1  i) \<or>
-(\<exists> i. i\<le>N\<and>r=n_RecvGntS2  i) \<or>
-(\<exists> i. i\<le>N\<and>r=n_SendGntE3  i) \<or>
-(\<exists> i. i\<le>N\<and>r=n_SendGntS4  i) \<or>
-(\<exists> i. i\<le>N\<and>r=n_RecvInvAck5  i) \<or>
-(\<exists> i. i\<le>N\<and>r=n_RecvInvAck6  i) \<or>
-(\<exists> i. i\<le>N\<and>r=n_SendInvAck7  i) \<or>
-(\<exists> i. i\<le>N\<and>r=n_SendInvAck8  i) \<or>
-(\<exists> i. i\<le>N\<and>r=n_SendInv9  i) \<or>
-(\<exists> i. i\<le>N\<and>r=n_SendInv10  i) \<or>
-(\<exists> i. i\<le>N\<and>r=n_RecvReqE11  i) \<or>
-(\<exists> i. i\<le>N\<and>r=n_RecvReqS12  i) \<or>
-(\<exists> i. i\<le>N\<and>r=n_SendReqE13  i) \<or>
-(\<exists> i. i\<le>N\<and>r=n_SendReqE14  i) \<or>
-(\<exists> i. i\<le>N\<and>r=n_SendReqS15  i) \<or>
-(\<exists> i. i\<le>N\<and>r=n_Store16  i)
-}"
+text \<open>initial state \<close>
 
 definition initSpec0::"nat \<Rightarrow> formula" where [simp]:
-"initSpec0 N\<equiv> (andList (map (\<lambda>i. (eqn (IVar (Para (''Chan1.Cmd :'') i)) (Const Empty)) ) (down N) ))"
+"initSpec0 N\<equiv> (\<forall>\<^sub>fi. (IVar (Para (''Chan1.Cmd'') i)) =\<^sub>f  (Const Empty) ) N "
 
 definition initSpec1::"nat \<Rightarrow> formula" where [simp]:
-"initSpec1 N\<equiv> (andList (map (\<lambda>i. (eqn (IVar (Para (''Chan2.Cmd :'') i)) (Const Empty)) ) (down N) ))"
+"initSpec1 N\<equiv> (\<forall>\<^sub>fi. (IVar (Para (''Chan2.Cmd'') i)) =\<^sub>f  (Const Empty) ) N "
 
 definition initSpec2::"nat \<Rightarrow> formula" where [simp]:
-"initSpec2 N\<equiv> (andList (map (\<lambda>i. (eqn (IVar (Para (''Chan3.Cmd :'') i)) (Const Empty)) ) (down N) ))"
+"initSpec2 N\<equiv> (\<forall>\<^sub>fi. (IVar (Para (''Chan3.Cmd'') i)) =\<^sub>f  (Const Empty) ) N "
 
 definition initSpec3::"nat \<Rightarrow> formula" where [simp]:
-"initSpec3 N\<equiv> (andList (map (\<lambda>i. (eqn (IVar (Para (''Cache.State :'') i)) (Const I)) ) (down N) ))"
+"initSpec3 N\<equiv> (\<forall>\<^sub>fi. (IVar (Para (''Cache.State'') i)) =\<^sub>f  (Const I) ) N "
 
 definition initSpec4::"nat \<Rightarrow> formula" where [simp]:
-"initSpec4 N\<equiv> (andList (map (\<lambda>i. (eqn (IVar (Para (''InvSet'') i)) (Const false)) ) (down N) ))"
+"initSpec4 N\<equiv> (\<forall>\<^sub>fi. (IVar (Para (''InvSet'') i)) =\<^sub>f  (Const false) ) N "
 
 definition initSpec5::"nat \<Rightarrow> formula" where [simp]:
-"initSpec5 N\<equiv> (andList (map (\<lambda>i. (eqn (IVar (Para (''ShrSet'') i)) (Const false)) ) (down N) ))"
+"initSpec5 N\<equiv> (\<forall>\<^sub>fi. (IVar (Para (''ShrSet'') i)) =\<^sub>f  (Const false) ) N "
 
 definition initSpec6::"nat \<Rightarrow> formula" where [simp]:
-"initSpec6 N \<equiv> (eqn (IVar (Ident ''ExGntd :'')) (Const false)) "
+"initSpec6 N \<equiv> (IVar (Ident ''ExGntd'')) =\<^sub>f  (Const false) "
 
 definition initSpec7::"nat \<Rightarrow> formula" where [simp]:
-"initSpec7 N \<equiv> (eqn (IVar (Ident ''CurCmd :'')) (Const Empty)) "
+"initSpec7 N \<equiv> (IVar (Ident ''CurCmd'')) =\<^sub>f  (Const Empty) "
 
-definition initSpec8::"nat \<Rightarrow> formula" where [simp]:
-"initSpec8 N \<equiv> (eqn (IVar (Ident ''MemData :'')) (IVar(Ident ''d''))) "
+lemma absInitSpec:
+assumes "M \<le> N"
+shows "absTransfForm M (initSpec0 N) = initSpec0 M"
+"absTransfForm M (initSpec1 N) = initSpec1 M"
+"absTransfForm M (initSpec2 N) = initSpec2 M"
+"absTransfForm M (initSpec3 N) = initSpec3 M"
+"absTransfForm M (initSpec4 N) = initSpec4 M"
+"absTransfForm M (initSpec5 N) = initSpec5 M"
+"absTransfForm M initSpec6 = initSpec6"
+"absTransfForm M initSpec7 = initSpec7"
+unfolding initSpec0_def initSpec1_def initSpec2_def initSpec3_def initSpec4_def initSpec5_def initSpec6_def initSpec7_def 
+using assms by auto
 
-definition initSpec9::"nat \<Rightarrow> formula" where [simp]:
-"initSpec9 N \<equiv> (eqn (IVar (Ident ''AuxData :'')) (IVar(Ident ''d''))) "
 
-definition allInitSpecs::"nat \<Rightarrow> formula list" where [simp]:
+definition allInitSpecs::"nat \<Rightarrow> formula list" where
 "allInitSpecs N \<equiv> [
 (initSpec0 N),
 (initSpec1 N),
@@ -169,367 +67,562 @@ definition allInitSpecs::"nat \<Rightarrow> formula list" where [simp]:
 (initSpec3 N),
 (initSpec4 N),
 (initSpec5 N),
-(initSpec6 N),
-(initSpec7 N),
-(initSpec8 N),
-(initSpec9 N)
+(initSpec6),
+(initSpec7)
 ]"
+lemma symPreds0[intro]:
+  "symPredSet' N ({(initSpec0 N)} )"
+unfolding initSpec0_def
+    apply (rule symPredSetForall)
+  unfolding symParamForm_def by auto
+
+lemma symPreds1[intro]:
+  "symPredSet' N ({(initSpec1 N)} )"
+unfolding initSpec1_def
+    apply (rule symPredSetForall)
+  unfolding symParamForm_def by auto
+
+lemma symPreds2[intro]:
+  "symPredSet' N ({(initSpec2 N)} )"
+unfolding initSpec2_def
+    apply (rule symPredSetForall)
+  unfolding symParamForm_def by auto
+
+lemma symPreds3[intro]:
+  "symPredSet' N ({(initSpec3 N)} )"
+unfolding initSpec3_def
+    apply (rule symPredSetForall)
+  unfolding symParamForm_def by auto
+
+lemma symPreds4[intro]:
+  "symPredSet' N ({(initSpec4 N)} )"
+unfolding initSpec4_def
+    apply (rule symPredSetForall)
+  unfolding symParamForm_def by auto
+
+lemma symPreds5[intro]:
+  "symPredSet' N ({(initSpec5 N)} )"
+unfolding initSpec5_def
+    apply (rule symPredSetForall)
+  unfolding symParamForm_def by auto
+
+lemma symPreds6[intro]:
+  "symPredSet' N ({(initSpec6 )} )"
+  unfolding symPredSet'_def initSpec6_def by auto
+
+lemma symPreds7[intro]:
+  "symPredSet' N ({(initSpec7 )} )"
+  unfolding symPredSet'_def initSpec7_def by auto
+
+lemma symPreds:
+  "symPredSet' N (    {(initSpec0 N)} \<union>
+    {(initSpec1 N)} \<union>
+    {(initSpec2 N)} \<union>
+    {(initSpec3 N)} \<union>
+    {(initSpec4 N)} \<union>
+    {(initSpec5 N)} \<union>
+    {initSpec6} \<union>
+    {initSpec7})"
+
+  apply (meson symPreds0 symPreds1 symPreds2 symPreds3 symPreds4 symPreds5 symPreds6 symPreds7 
+symPredsUnion)
+  done
+
+lemma symPreds':
+"symPredSet' N (set (allInitSpecs N))"
+  proof -
+    have b1:"(set (allInitSpecs N)) =
+    {(initSpec0 N)}\<union>
+    {(initSpec1 N)}\<union>
+    {(initSpec2 N)}\<union>
+    {(initSpec3 N)}\<union>
+    {(initSpec4 N)}\<union>
+    {(initSpec5 N)}\<union>
+    {(initSpec6 N)}\<union>
+    {(initSpec7 N)}" (is "?LHS=?RHS")
+      using allInitSpecs_def by auto
+    have b2:"symPredSet' N ?RHS"
+      using symPreds by blast
+    show "symPredSet' N (set (allInitSpecs N))"
+      using b1 b2 by auto
+  qed
+
+definition n_RecvGntE1::"nat \<Rightarrow> rule" where 
+"n_RecvGntE1  i\<equiv>
+(IVar (Para (''Chan2.Cmd'') i)) =\<^sub>f  (Const GntE) 
+   \<triangleright>
+(assign (Para (''Cache.State'') i, (Const E)))||
+(assign (Para (''Cache.Data'') i, (IVar (Para (''Chan2.Data'') i))))||
+(assign (Para (''Chan2.Cmd'') i, (Const Empty)))"
+
+lemma symRecvGntE1:
+  "symParamRule N n_RecvGntE1"
+  "wellFormedStatement N (act (n_RecvGntE1 i))"
+  "absTransfRule M (n_RecvGntE1 i) = (if i \<le> M then n_RecvGntE1 i else chaos
+\<triangleright> skip)"
+  unfolding n_RecvGntE1_def symParamRule_def by auto
+
+definition n_RecvGntS2::"nat \<Rightarrow> rule" where 
+"n_RecvGntS2  i\<equiv>
+(IVar (Para (''Chan2.Cmd'') i)) =\<^sub>f  (Const GntS) 
+   \<triangleright>
+(assign (Para (''Cache.State'') i, (Const S)))||
+(assign (Para (''Cache.Data'') i, (IVar (Para (''Chan2.Data'') i))))||
+(assign (Para (''Chan2.Cmd'') i, (Const Empty)))"
+
+lemma symRecvGntS2:
+  "symParamRule N n_RecvGntS2"
+  "wellFormedStatement N (act (n_RecvGntS2 i))"
+  "absTransfRule M (n_RecvGntS2 i) = (if i \<le> M then n_RecvGntS2 i else chaos
+\<triangleright> skip)"
+  unfolding n_RecvGntS2_def symParamRule_def by auto
+
+definition n_SendGntE3::"nat \<Rightarrow> nat \<Rightarrow> rule" where 
+"n_SendGntE3  i N\<equiv>
+(IVar (Ident ''CurCmd''))  =\<^sub>f (Const ReqE)  \<and>\<^sub>f
+(IVar (Ident ''CurPtr''))  =\<^sub>f (Const (index i))  \<and>\<^sub>f
+(IVar (Para (''Chan2.Cmd'') i)) =\<^sub>f  (Const Empty)  \<and>\<^sub>f
+(IVar (Ident ''ExGntd''))  =\<^sub>f (Const false)  \<and>\<^sub>f
+(\<forall>\<^sub>fj. (IVar (Para (''ShrSet'') j)) =\<^sub>f  (Const false) )) M
+   \<triangleright>
+(assign (Para (''Chan2.Cmd'') i, (Const GntE)))||
+(assign (Para (''Chan2.Data'') i, (IVar (Ident ''MemData''))))||
+(assign (Para (''ShrSet'') i, (Const true)))||
+(assign ((Ident ''ExGntd''), (Const true)))||
+(assign ((Ident ''CurCmd''), (Const Empty)))"
+
+lemma symSendGntE3:
+  "symParamRule N n_SendGntE3"
+  "wellFormedStatement N (act (n_SendGntE3 i))"
+  "absTransfRule M (n_SendGntE3 i) = (if i \<le> M then n_SendGntE3 i else chaos
+\<triangleright> skip)"
+  unfolding n_SendGntE3_def symParamRule_def by auto
+
+definition n_SendGntS4::"nat \<Rightarrow> rule" where 
+"n_SendGntS4  i\<equiv>
+(IVar (Ident ''CurCmd''))  =\<^sub>f (Const ReqS)  \<and>\<^sub>f
+(IVar (Ident ''CurPtr''))  =\<^sub>f (Const (index i))  \<and>\<^sub>f
+(IVar (Para (''Chan2.Cmd'') i)) =\<^sub>f  (Const Empty)  \<and>\<^sub>f
+(IVar (Ident ''ExGntd''))  =\<^sub>f (Const false) 
+   \<triangleright>
+(assign (Para (''Chan2.Cmd'') i, (Const GntS)))||
+(assign (Para (''Chan2.Data'') i, (IVar (Ident ''MemData''))))||
+(assign (Para (''ShrSet'') i, (Const true)))||
+(assign ((Ident ''CurCmd''), (Const Empty)))"
+
+lemma symSendGntS4:
+  "symParamRule N n_SendGntS4"
+  "wellFormedStatement N (act (n_SendGntS4 i))"
+  "absTransfRule M (n_SendGntS4 i) = (if i \<le> M then n_SendGntS4 i else chaos
+\<triangleright> skip)"
+  unfolding n_SendGntS4_def symParamRule_def by auto
+
+definition n_RecvInvAck5::"nat \<Rightarrow> rule" where 
+"n_RecvInvAck5  i\<equiv>
+(IVar (Para (''Chan3.Cmd'') i)) =\<^sub>f  (Const InvAck)  \<and>\<^sub>f
+\<not>\<^sub>f (IVar (Ident ''CurCmd'')) =\<^sub>f  (Const Empty)  \<and>\<^sub>f
+(IVar (Ident ''ExGntd''))  =\<^sub>f (Const true) 
+   \<triangleright>
+(assign (Para (''Chan3.Cmd'') i, (Const Empty)))||
+(assign (Para (''ShrSet'') i, (Const false)))||
+(assign ((Ident ''ExGntd''), (Const false)))||
+(assign ((Ident ''MemData''), (IVar (Para (''Chan3.Data'') i))))"
+
+lemma symRecvInvAck5:
+  "symParamRule N n_RecvInvAck5"
+  "wellFormedStatement N (act (n_RecvInvAck5 i))"
+  "absTransfRule M (n_RecvInvAck5 i) = (if i \<le> M then n_RecvInvAck5 i else chaos
+\<triangleright> skip)"
+  unfolding n_RecvInvAck5_def symParamRule_def by auto
+
+definition n_RecvInvAck6::"nat \<Rightarrow> rule" where 
+"n_RecvInvAck6  i\<equiv>
+(IVar (Para (''Chan3.Cmd'') i)) =\<^sub>f  (Const InvAck)  \<and>\<^sub>f
+\<not>\<^sub>f (IVar (Ident ''CurCmd'')) =\<^sub>f  (Const Empty)  \<and>\<^sub>f
+\<not>\<^sub>f (IVar (Ident ''ExGntd'')) =\<^sub>f  (Const true) 
+   \<triangleright>
+(assign (Para (''Chan3.Cmd'') i, (Const Empty)))||
+(assign (Para (''ShrSet'') i, (Const false)))"
+
+lemma symRecvInvAck6:
+  "symParamRule N n_RecvInvAck6"
+  "wellFormedStatement N (act (n_RecvInvAck6 i))"
+  "absTransfRule M (n_RecvInvAck6 i) = (if i \<le> M then n_RecvInvAck6 i else chaos
+\<triangleright> skip)"
+  unfolding n_RecvInvAck6_def symParamRule_def by auto
+
+definition n_SendInvAck7::"nat \<Rightarrow> rule" where 
+"n_SendInvAck7  i\<equiv>
+(IVar (Para (''Chan2.Cmd'') i)) =\<^sub>f  (Const Inv)  \<and>\<^sub>f
+(IVar (Para (''Chan3.Cmd'') i)) =\<^sub>f  (Const Empty)  \<and>\<^sub>f
+(IVar (Para (''Cache.State'') i)) =\<^sub>f  (Const E) 
+   \<triangleright>
+(assign (Para (''Chan2.Cmd'') i, (Const Empty)))||
+(assign (Para (''Chan3.Cmd'') i, (Const InvAck)))||
+(assign (Para (''Chan3.Data'') i, (IVar (Para (''Cache.Data'') i))))||
+(assign (Para (''Cache.State'') i, (Const I)))"
+
+lemma symSendInvAck7:
+  "symParamRule N n_SendInvAck7"
+  "wellFormedStatement N (act (n_SendInvAck7 i))"
+  "absTransfRule M (n_SendInvAck7 i) = (if i \<le> M then n_SendInvAck7 i else chaos
+\<triangleright> skip)"
+  unfolding n_SendInvAck7_def symParamRule_def by auto
+
+definition n_SendInvAck8::"nat \<Rightarrow> rule" where 
+"n_SendInvAck8  i\<equiv>
+(IVar (Para (''Chan2.Cmd'') i)) =\<^sub>f  (Const Inv)  \<and>\<^sub>f
+(IVar (Para (''Chan3.Cmd'') i)) =\<^sub>f  (Const Empty)  \<and>\<^sub>f
+\<not>\<^sub>f (IVar (Para (''Cache.State'') i)) =\<^sub>f  (Const E) 
+   \<triangleright>
+(assign (Para (''Chan2.Cmd'') i, (Const Empty)))||
+(assign (Para (''Chan3.Cmd'') i, (Const InvAck)))||
+(assign (Para (''Cache.State'') i, (Const I)))"
+
+lemma symSendInvAck8:
+  "symParamRule N n_SendInvAck8"
+  "wellFormedStatement N (act (n_SendInvAck8 i))"
+  "absTransfRule M (n_SendInvAck8 i) = (if i \<le> M then n_SendInvAck8 i else chaos
+\<triangleright> skip)"
+  unfolding n_SendInvAck8_def symParamRule_def by auto
+
+definition n_SendInv9::"nat \<Rightarrow> rule" where 
+"n_SendInv9  i\<equiv>
+(IVar (Para (''Chan2.Cmd'') i)) =\<^sub>f  (Const Empty)  \<and>\<^sub>f
+(IVar (Para (''InvSet'') i)) =\<^sub>f  (Const true)  \<and>\<^sub>f
+(IVar (Ident ''CurCmd''))  =\<^sub>f (Const ReqE) 
+   \<triangleright>
+(assign (Para (''Chan2.Cmd'') i, (Const Inv)))||
+(assign (Para (''InvSet'') i, (Const false)))"
+
+lemma symSendInv9:
+  "symParamRule N n_SendInv9"
+  "wellFormedStatement N (act (n_SendInv9 i))"
+  "absTransfRule M (n_SendInv9 i) = (if i \<le> M then n_SendInv9 i else chaos
+\<triangleright> skip)"
+  unfolding n_SendInv9_def symParamRule_def by auto
+
+definition n_SendInv10::"nat \<Rightarrow> rule" where 
+"n_SendInv10  i\<equiv>
+(IVar (Para (''Chan2.Cmd'') i)) =\<^sub>f  (Const Empty)  \<and>\<^sub>f
+(IVar (Para (''InvSet'') i)) =\<^sub>f  (Const true)  \<and>\<^sub>f
+(IVar (Ident ''CurCmd''))  =\<^sub>f (Const ReqS)  \<and>\<^sub>f
+(IVar (Ident ''ExGntd''))  =\<^sub>f (Const true) 
+   \<triangleright>
+(assign (Para (''Chan2.Cmd'') i, (Const Inv)))||
+(assign (Para (''InvSet'') i, (Const false)))"
+
+lemma symSendInv10:
+  "symParamRule N n_SendInv10"
+  "wellFormedStatement N (act (n_SendInv10 i))"
+  "absTransfRule M (n_SendInv10 i) = (if i \<le> M then n_SendInv10 i else chaos
+\<triangleright> skip)"
+  unfolding n_SendInv10_def symParamRule_def by auto
+
+definition n_RecvReqE11::"nat \<Rightarrow> nat \<Rightarrow> rule" where 
+"n_RecvReqE11  i N\<equiv>
+(IVar (Ident ''CurCmd''))  =\<^sub>f (Const Empty)  \<and>\<^sub>f
+(IVar (Para (''Chan1.Cmd'') i)) =\<^sub>f  (Const ReqE) 
+   \<triangleright>
+(assign ((Ident ''CurCmd''), (Const ReqE)))||
+(assign ((Ident ''CurPtr''), (Const (index i))))||
+(assign (Para (''Chan1.Cmd'') i, (Const Empty)))||
+(parallelList (map (\<lambda>j. (assign (Para (''InvSet'') j, (IVar (Para (''ShrSet'') j))))) (down N)))"
+
+lemma symRecvReqE11:
+  "symParamRule N n_RecvReqE11"
+  "wellFormedStatement N (act (n_RecvReqE11 i))"
+  "absTransfRule M (n_RecvReqE11 i) = (if i \<le> M then n_RecvReqE11 i else chaos
+\<triangleright> skip)"
+  unfolding n_RecvReqE11_def symParamRule_def by auto
+
+definition n_RecvReqS12::"nat \<Rightarrow> nat \<Rightarrow> rule" where 
+"n_RecvReqS12  i N\<equiv>
+(IVar (Ident ''CurCmd''))  =\<^sub>f (Const Empty)  \<and>\<^sub>f
+(IVar (Para (''Chan1.Cmd'') i)) =\<^sub>f  (Const ReqS) 
+   \<triangleright>
+(assign ((Ident ''CurCmd''), (Const ReqS)))||
+(assign ((Ident ''CurPtr''), (Const (index i))))||
+(assign (Para (''Chan1.Cmd'') i, (Const Empty)))||
+(parallelList (map (\<lambda>j. (assign (Para (''InvSet'') j, (IVar (Para (''ShrSet'') j))))) (down N)))"
+
+lemma symRecvReqS12:
+  "symParamRule N n_RecvReqS12"
+  "wellFormedStatement N (act (n_RecvReqS12 i))"
+  "absTransfRule M (n_RecvReqS12 i) = (if i \<le> M then n_RecvReqS12 i else chaos
+\<triangleright> skip)"
+  unfolding n_RecvReqS12_def symParamRule_def by auto
+
+definition n_SendReqE13::"nat \<Rightarrow> rule" where 
+"n_SendReqE13  i\<equiv>
+(IVar (Para (''Chan1.Cmd'') i)) =\<^sub>f  (Const Empty)  \<and>\<^sub>f
+(IVar (Para (''Cache.State'') i)) =\<^sub>f  (Const I) 
+   \<triangleright>
+(assign (Para (''Chan1.Cmd'') i, (Const ReqE)))"
+
+lemma symSendReqE13:
+  "symParamRule N n_SendReqE13"
+  "wellFormedStatement N (act (n_SendReqE13 i))"
+  "absTransfRule M (n_SendReqE13 i) = (if i \<le> M then n_SendReqE13 i else chaos
+\<triangleright> skip)"
+  unfolding n_SendReqE13_def symParamRule_def by auto
+
+definition n_SendReqE14::"nat \<Rightarrow> rule" where 
+"n_SendReqE14  i\<equiv>
+(IVar (Para (''Chan1.Cmd'') i)) =\<^sub>f  (Const Empty)  \<and>\<^sub>f
+(IVar (Para (''Cache.State'') i)) =\<^sub>f  (Const S) 
+   \<triangleright>
+(assign (Para (''Chan1.Cmd'') i, (Const ReqE)))"
+
+lemma symSendReqE14:
+  "symParamRule N n_SendReqE14"
+  "wellFormedStatement N (act (n_SendReqE14 i))"
+  "absTransfRule M (n_SendReqE14 i) = (if i \<le> M then n_SendReqE14 i else chaos
+\<triangleright> skip)"
+  unfolding n_SendReqE14_def symParamRule_def by auto
+
+definition n_SendReqS15::"nat \<Rightarrow> rule" where 
+"n_SendReqS15  i\<equiv>
+(IVar (Para (''Chan1.Cmd'') i)) =\<^sub>f  (Const Empty)  \<and>\<^sub>f
+(IVar (Para (''Cache.State'') i)) =\<^sub>f  (Const I) 
+   \<triangleright>
+(assign (Para (''Chan1.Cmd'') i, (Const ReqS)))"
+
+lemma symSendReqS15:
+  "symParamRule N n_SendReqS15"
+  "wellFormedStatement N (act (n_SendReqS15 i))"
+  "absTransfRule M (n_SendReqS15 i) = (if i \<le> M then n_SendReqS15 i else chaos
+\<triangleright> skip)"
+  unfolding n_SendReqS15_def symParamRule_def by auto
+
+definition n_Store16::"nat \<Rightarrow> rule" where 
+"n_Store16  i\<equiv>
+(IVar (Para (''Cache.State'') i)) =\<^sub>f  (Const E) 
+   \<triangleright>
+(assign (Para (''Cache.Data'') i, (IVar(Ident ''d''))))||
+(assign ((Ident ''AuxData''), (IVar(Ident ''d''))))"
+
+lemma symStore16:
+  "symParamRule N n_Store16"
+  "wellFormedStatement N (act (n_Store16 i))"
+  "absTransfRule M (n_Store16 i) = (if i \<le> M then n_Store16 i else chaos
+\<triangleright> skip)"
+  unfolding n_Store16_def symParamRule_def by auto
+
+subsection \<open>Putting everything together ---definition of rules\<close>
+
+definition n_RecvGntE1s::" nat\<Rightarrow>rule set" where 
+  "n_RecvGntE1s N== oneParamCons N  n_RecvGntE1"
+
+definition n_RecvGntS2s::" nat\<Rightarrow>rule set" where 
+  "n_RecvGntS2s N== oneParamCons N  n_RecvGntS2"
+
+definition n_SendGntE3s::" nat\<Rightarrow>rule set" where 
+  "n_SendGntE3s N== oneParamCons N  n_SendGntE3"
+
+definition n_SendGntS4s::" nat\<Rightarrow>rule set" where 
+  "n_SendGntS4s N== oneParamCons N  n_SendGntS4"
+
+definition n_RecvInvAck5s::" nat\<Rightarrow>rule set" where 
+  "n_RecvInvAck5s N== oneParamCons N  n_RecvInvAck5"
+
+definition n_RecvInvAck6s::" nat\<Rightarrow>rule set" where 
+  "n_RecvInvAck6s N== oneParamCons N  n_RecvInvAck6"
+
+definition n_SendInvAck7s::" nat\<Rightarrow>rule set" where 
+  "n_SendInvAck7s N== oneParamCons N  n_SendInvAck7"
+
+definition n_SendInvAck8s::" nat\<Rightarrow>rule set" where 
+  "n_SendInvAck8s N== oneParamCons N  n_SendInvAck8"
+
+definition n_SendInv9s::" nat\<Rightarrow>rule set" where 
+  "n_SendInv9s N== oneParamCons N  n_SendInv9"
+
+definition n_SendInv10s::" nat\<Rightarrow>rule set" where 
+  "n_SendInv10s N== oneParamCons N  n_SendInv10"
+
+definition n_RecvReqE11s::" nat\<Rightarrow>rule set" where 
+  "n_RecvReqE11s N== oneParamCons N  n_RecvReqE11"
+
+definition n_RecvReqS12s::" nat\<Rightarrow>rule set" where 
+  "n_RecvReqS12s N== oneParamCons N  n_RecvReqS12"
+
+definition n_SendReqE13s::" nat\<Rightarrow>rule set" where 
+  "n_SendReqE13s N== oneParamCons N  n_SendReqE13"
+
+definition n_SendReqE14s::" nat\<Rightarrow>rule set" where 
+  "n_SendReqE14s N== oneParamCons N  n_SendReqE14"
+
+definition n_SendReqS15s::" nat\<Rightarrow>rule set" where 
+  "n_SendReqS15s N== oneParamCons N  n_SendReqS15"
+
+definition n_Store16s::" nat\<Rightarrow>rule set" where 
+  "n_Store16s N== oneParamCons N  n_Store16"
+
+definition rules'::"nat \<Rightarrow> rule set" where [simp]:
+"rules' N \<equiv>  (n_RecvGntE1s N) \<union>
+ (n_RecvGntS2s N) \<union>
+ (n_SendGntE3s N) \<union>
+ (n_SendGntS4s N) \<union>
+ (n_RecvInvAck5s N) \<union>
+ (n_RecvInvAck6s N) \<union>
+ (n_SendInvAck7s N) \<union>
+ (n_SendInvAck8s N) \<union>
+ (n_SendInv9s N) \<union>
+ (n_SendInv10s N) \<union>
+ (n_RecvReqE11s N) \<union>
+ (n_RecvReqS12s N) \<union>
+ (n_SendReqE13s N) \<union>
+ (n_SendReqE14s N) \<union>
+ (n_SendReqS15s N) \<union>
+ (n_Store16s N) 
+"
+
+lemma n_RecvGntE1sIsSym:
+  "symProtRules' N (n_RecvGntE1s N)"
+  using symRecvGntE1(1) n_RecvGntE1s_def symParaRuleInfSymRuleSet by auto
+
+lemma n_RecvGntS2sIsSym:
+  "symProtRules' N (n_RecvGntS2s N)"
+  using symRecvGntS2(1) n_RecvGntS2s_def symParaRuleInfSymRuleSet by auto
+
+lemma n_SendGntE3sIsSym:
+  "symProtRules' N (n_SendGntE3s N)"
+  using symSendGntE3(1) n_SendGntE3s_def symParaRuleInfSymRuleSet by auto
+
+lemma n_SendGntS4sIsSym:
+  "symProtRules' N (n_SendGntS4s N)"
+  using symSendGntS4(1) n_SendGntS4s_def symParaRuleInfSymRuleSet by auto
+
+lemma n_RecvInvAck5sIsSym:
+  "symProtRules' N (n_RecvInvAck5s N)"
+  using symRecvInvAck5(1) n_RecvInvAck5s_def symParaRuleInfSymRuleSet by auto
+
+lemma n_RecvInvAck6sIsSym:
+  "symProtRules' N (n_RecvInvAck6s N)"
+  using symRecvInvAck6(1) n_RecvInvAck6s_def symParaRuleInfSymRuleSet by auto
+
+lemma n_SendInvAck7sIsSym:
+  "symProtRules' N (n_SendInvAck7s N)"
+  using symSendInvAck7(1) n_SendInvAck7s_def symParaRuleInfSymRuleSet by auto
+
+lemma n_SendInvAck8sIsSym:
+  "symProtRules' N (n_SendInvAck8s N)"
+  using symSendInvAck8(1) n_SendInvAck8s_def symParaRuleInfSymRuleSet by auto
+
+lemma n_SendInv9sIsSym:
+  "symProtRules' N (n_SendInv9s N)"
+  using symSendInv9(1) n_SendInv9s_def symParaRuleInfSymRuleSet by auto
+
+lemma n_SendInv10sIsSym:
+  "symProtRules' N (n_SendInv10s N)"
+  using symSendInv10(1) n_SendInv10s_def symParaRuleInfSymRuleSet by auto
+
+lemma n_RecvReqE11sIsSym:
+  "symProtRules' N (n_RecvReqE11s N)"
+  using symRecvReqE11(1) n_RecvReqE11s_def symParaRuleInfSymRuleSet by auto
+
+lemma n_RecvReqS12sIsSym:
+  "symProtRules' N (n_RecvReqS12s N)"
+  using symRecvReqS12(1) n_RecvReqS12s_def symParaRuleInfSymRuleSet by auto
+
+lemma n_SendReqE13sIsSym:
+  "symProtRules' N (n_SendReqE13s N)"
+  using symSendReqE13(1) n_SendReqE13s_def symParaRuleInfSymRuleSet by auto
+
+lemma n_SendReqE14sIsSym:
+  "symProtRules' N (n_SendReqE14s N)"
+  using symSendReqE14(1) n_SendReqE14s_def symParaRuleInfSymRuleSet by auto
+
+lemma n_SendReqS15sIsSym:
+  "symProtRules' N (n_SendReqS15s N)"
+  using symSendReqS15(1) n_SendReqS15s_def symParaRuleInfSymRuleSet by auto
+
+lemma n_Store16sIsSym:
+  "symProtRules' N (n_Store16s N)"
+  using symStore16(1) n_Store16s_def symParaRuleInfSymRuleSet by auto
+
+lemma rulesSym':
+  shows "symProtRules' N (rules' N)"
+  using n_RecvGntE1sIsSym n_RecvGntS2sIsSym n_SendGntE3sIsSym n_SendGntS4sIsSym n_RecvInvAck5sIsSym n_RecvInvAck6sIsSym n_SendInvAck7sIsSym n_SendInvAck8sIsSym n_SendInv9sIsSym n_SendInv10sIsSym n_RecvReqE11sIsSym n_RecvReqS12sIsSym n_SendReqE13sIsSym n_SendReqE14sIsSym n_SendReqS15sIsSym n_Store16sIsSym rules'_def symProtRulesUnion by presburger 
 
 
-definition inv_0 :: "nat \<Rightarrow> nat \<Rightarrow> formula" where [simp]:
-	"inv_0 i j \<equiv>
-		implyForm (andList [(neg (eqn (Const (index i)) (Const (index j)))), (eqn (IVar (Para (''Chan2.Cmd'') i)) (Const Inv)) , (eqn (IVar (Para (''Cache.State!'') i)) (Const E)) ])
-(eqn (IVar (Ident ''ExGntd'')) (Const false)) "
-
-definition inv_1 :: "nat \<Rightarrow> nat \<Rightarrow> formula" where [simp]:
-	"inv_1 i j \<equiv>
-		implyForm (andForm (neg (eqn (Const (index i)) (Const (index j)))) (eqn (IVar (Para (''Cache.State'') i)) (Const S)) )
-(eqn (IVar (Ident ''MemData'')) (IVar (Ident ''AuxData''))) "
-
-definition inv_2 :: "nat \<Rightarrow> nat \<Rightarrow> formula" where [simp]:
-	"inv_2 i j \<equiv>
-		implyForm (andForm (neg (eqn (Const (index i)) (Const (index j)))) (eqn (IVar (Para (''Chan2.Cmd'') i)) (Const GntS)) )
-(eqn (IVar (Ident ''ExGntd'')) (Const false)) "
-
-definition inv_3 :: "nat \<Rightarrow> nat \<Rightarrow> formula" where [simp]:
-	"inv_3 i j \<equiv>
-		implyForm (andList [(neg (eqn (Const (index i)) (Const (index j)))), (eqn (IVar (Para (''Chan2.Cmd'') i)) (Const Inv)) , (eqn (IVar (Para (''Cache.State!'') i)) (Const E)) ])
-(eqn (IVar (Ident ''CurCmd!'')) (Const ReqS)) "
-
-definition inv_4 :: "nat \<Rightarrow> nat \<Rightarrow> formula" where [simp]:
-	"inv_4 i j \<equiv>
-		implyForm (andForm (neg (eqn (Const (index i)) (Const (index j)))) (eqn (IVar (Para (''Chan2.Cmd'') i)) (Const GntE)) )
-(eqn (IVar (Ident ''ExGntd'')) (Const true)) "
-
-definition inv_5 :: "nat \<Rightarrow> nat \<Rightarrow> formula" where [simp]:
-	"inv_5 i j \<equiv>
-		implyForm (andList [(neg (eqn (Const (index i)) (Const (index j)))), (eqn (IVar (Ident ''ExGntd'')) (Const true)) , (eqn (IVar (Para (''Chan3.Cmd'') i)) (Const InvAck)) ])
-(eqn (IVar (Para (''Chan3.Data'') i)) (IVar (Ident ''AuxData''))) "
-
-definition inv_6 :: "nat \<Rightarrow> nat \<Rightarrow> formula" where [simp]:
-	"inv_6 i j \<equiv>
-		implyForm (andList [(neg (eqn (Const (index i)) (Const (index j)))), (eqn (IVar (Para (''Chan2.Cmd'') i)) (Const Inv)) , (eqn (IVar (Para (''Cache.State!'') i)) (Const E)) ])
-(eqn (IVar (Ident ''MemData'')) (IVar (Ident ''AuxData''))) "
-
-definition inv_7 :: "nat \<Rightarrow> nat \<Rightarrow> formula" where [simp]:
-	"inv_7 i j \<equiv>
-		implyForm (andList [(neg (eqn (Const (index i)) (Const (index j)))), (eqn (IVar (Para (''InvSet'') i)) (Const true)) , (eqn (IVar (Ident ''ExGntd'')) (Const true)) ])
-(eqn (IVar (Ident ''CurCmd!'')) (Const Empty)) "
-
-definition inv_8 :: "nat \<Rightarrow> nat \<Rightarrow> formula" where [simp]:
-	"inv_8 i j \<equiv>
-		implyForm (andForm (neg (eqn (Const (index i)) (Const (index j)))) (eqn (IVar (Para (''Cache.State'') i)) (Const S)) )
-(eqn (IVar (Ident ''ExGntd'')) (Const false)) "
-
-definition inv_9 :: "nat \<Rightarrow> nat \<Rightarrow> formula" where [simp]:
-	"inv_9 i j \<equiv>
-		implyForm (andForm (neg (eqn (Const (index i)) (Const (index j)))) (eqn (IVar (Para (''Chan2.Cmd'') i)) (Const Inv)) )
-(eqn (IVar (Ident ''CurCmd!'')) (Const Empty)) "
-
-definition inv_10 :: "nat \<Rightarrow> nat \<Rightarrow> formula" where [simp]:
-	"inv_10 i j \<equiv>
-		implyForm (andForm (neg (eqn (Const (index i)) (Const (index j)))) (eqn (IVar (Para (''Chan2.Cmd'') i)) (Const GntE)) )
-(eqn (IVar (Ident ''MemData'')) (IVar (Ident ''AuxData''))) "
-
-definition inv_11 :: "nat \<Rightarrow> nat \<Rightarrow> formula" where [simp]:
-	"inv_11 i j \<equiv>
-		implyForm (andForm (neg (eqn (Const (index i)) (Const (index j)))) (eqn (IVar (Para (''Cache.State'') i)) (Const E)) )
-(eqn (IVar (Ident ''ExGntd'')) (Const true)) "
-
-definition inv_12 :: "nat \<Rightarrow> nat \<Rightarrow> formula" where [simp]:
-	"inv_12 i j \<equiv>
-		implyForm (andForm (neg (eqn (Const (index i)) (Const (index j)))) (eqn (IVar (Para (''Chan2.Cmd'') i)) (Const GntS)) )
-(eqn (IVar (Ident ''MemData'')) (IVar (Ident ''AuxData''))) "
-
-definition inv_13 :: "nat \<Rightarrow> nat \<Rightarrow> formula" where [simp]:
-	"inv_13 i j \<equiv>
-		implyForm (andList [(neg (eqn (Const (index i)) (Const (index j)))), (eqn (IVar (Para (''Chan2.Cmd'') i)) (Const Inv)) , (eqn (IVar (Para (''Cache.State!'') i)) (Const E)) ])
-(eqn (IVar (Ident ''CurCmd'')) (Const ReqE)) "
-
-definition inv_14 :: "nat \<Rightarrow> nat \<Rightarrow> formula" where [simp]:
-	"inv_14 i j \<equiv>
-		implyForm (andForm (neg (eqn (Const (index i)) (Const (index j)))) (eqn (IVar (Para (''Chan3.Cmd'') i)) (Const InvAck)) )
-(eqn (IVar (Para (''Cache.State !'') j)) (Const E)) "
-
-definition inv_15 :: "nat \<Rightarrow> nat \<Rightarrow> formula" where [simp]:
-	"inv_15 i j \<equiv>
-		implyForm (andForm (neg (eqn (Const (index i)) (Const (index j)))) (eqn (IVar (Para (''InvSet'') i)) (Const true)) )
-(eqn (IVar (Para (''Cache.State !'') j)) (Const E)) "
-
-definition inv_16 :: "nat \<Rightarrow> nat \<Rightarrow> formula" where [simp]:
-	"inv_16 i j \<equiv>
-		implyForm (andList [(neg (eqn (Const (index i)) (Const (index j)))), (eqn (IVar (Para (''InvSet'') i)) (Const true)) , (eqn (IVar (Ident ''CurCmd'')) (Const ReqS)) ])
-(eqn (IVar (Para (''Chan3.Cmd'') j)) (Const Empty)) "
-
-definition inv_17 :: "nat \<Rightarrow> nat \<Rightarrow> formula" where [simp]:
-	"inv_17 i j \<equiv>
-		implyForm (andList [(neg (eqn (Const (index i)) (Const (index j)))), (eqn (IVar (Para (''InvSet'') i)) (Const true)) , (eqn (IVar (Ident ''ExGntd'')) (Const true)) ])
-(eqn (IVar (Para (''Cache.State'') j)) (Const I)) "
-
-definition inv_18 :: "nat \<Rightarrow> nat \<Rightarrow> formula" where [simp]:
-	"inv_18 i j \<equiv>
-		implyForm (andForm (neg (eqn (Const (index i)) (Const (index j)))) (eqn (IVar (Para (''Cache.State'') i)) (Const E)) )
-(eqn (IVar (Para (''Chan2.Cmd'') j)) (Const Empty)) "
-
-definition inv_19 :: "nat \<Rightarrow> nat \<Rightarrow> formula" where [simp]:
-	"inv_19 i j \<equiv>
-		implyForm (andList [(neg (eqn (Const (index i)) (Const (index j)))), (eqn (IVar (Para (''InvSet'') i)) (Const true)) , (eqn (IVar (Ident ''ExGntd'')) (Const true)) ])
-(eqn (IVar (Para (''InvSet'') j)) (Const false)) "
-
-definition inv_20 :: "nat \<Rightarrow> nat \<Rightarrow> formula" where [simp]:
-	"inv_20 i j \<equiv>
-		implyForm (andForm (neg (eqn (Const (index i)) (Const (index j)))) (eqn (IVar (Para (''Chan2.Cmd'') i)) (Const GntE)) )
-(eqn (IVar (Para (''InvSet'') j)) (Const false)) "
-
-definition inv_21 :: "nat \<Rightarrow> nat \<Rightarrow> formula" where [simp]:
-	"inv_21 i j \<equiv>
-		implyForm (andForm (neg (eqn (Const (index i)) (Const (index j)))) (eqn (IVar (Para (''Cache.State'') i)) (Const E)) )
-(eqn (IVar (Para (''Cache.State !'') j)) (Const S)) "
-
-definition inv_22 :: "nat \<Rightarrow> nat \<Rightarrow> formula" where [simp]:
-	"inv_22 i j \<equiv>
-		implyForm (andList [(neg (eqn (Const (index i)) (Const (index j)))), (eqn (IVar (Para (''InvSet'') i)) (Const true)) , (eqn (IVar (Ident ''ExGntd'')) (Const true)) ])
-(eqn (IVar (Para (''ShrSet'') j)) (Const false)) "
-
-definition inv_23 :: "nat \<Rightarrow> nat \<Rightarrow> formula" where [simp]:
-	"inv_23 i j \<equiv>
-		implyForm (andForm (neg (eqn (Const (index i)) (Const (index j)))) (eqn (IVar (Para (''Chan2.Cmd'') i)) (Const GntE)) )
-(eqn (IVar (Para (''Cache.State !'') j)) (Const E)) "
-
-definition inv_24 :: "nat \<Rightarrow> nat \<Rightarrow> formula" where [simp]:
-	"inv_24 i j \<equiv>
-		implyForm (andForm (neg (eqn (Const (index i)) (Const (index j)))) (eqn (IVar (Para (''Cache.State'') i)) (Const E)) )
-(eqn (IVar (Para (''Cache.State'') j)) (Const I)) "
-
-definition inv_25 :: "nat \<Rightarrow> nat \<Rightarrow> formula" where [simp]:
-	"inv_25 i j \<equiv>
-		implyForm (andForm (neg (eqn (Const (index i)) (Const (index j)))) (eqn (IVar (Para (''Cache.State'') i)) (Const E)) )
-(eqn (IVar (Para (''Chan2.Cmd !'') j)) (Const GntS)) "
-
-definition inv_26 :: "nat \<Rightarrow> nat \<Rightarrow> formula" where [simp]:
-	"inv_26 i j \<equiv>
-		implyForm (andForm (neg (eqn (Const (index i)) (Const (index j)))) (eqn (IVar (Para (''Chan2.Cmd'') i)) (Const GntE)) )
-(eqn (IVar (Para (''Chan2.Cmd'') j)) (Const Empty)) "
-
-definition inv_27 :: "nat \<Rightarrow> nat \<Rightarrow> formula" where [simp]:
-	"inv_27 i j \<equiv>
-		implyForm (andList [(neg (eqn (Const (index i)) (Const (index j)))), (eqn (IVar (Ident ''ExGntd'')) (Const true)) , (eqn (IVar (Para (''Chan3.Cmd'') i)) (Const InvAck)) ])
-(eqn (IVar (Para (''Cache.State'') j)) (Const I)) "
-
-definition inv_28 :: "nat \<Rightarrow> nat \<Rightarrow> formula" where [simp]:
-	"inv_28 i j \<equiv>
-		implyForm (andForm (neg (eqn (Const (index i)) (Const (index j)))) (eqn (IVar (Para (''Chan2.Cmd'') i)) (Const GntE)) )
-(eqn (IVar (Para (''Chan2.Cmd !'') j)) (Const GntS)) "
-
-definition inv_29 :: "nat \<Rightarrow> nat \<Rightarrow> formula" where [simp]:
-	"inv_29 i j \<equiv>
-		implyForm (andList [(neg (eqn (Const (index i)) (Const (index j)))), (eqn (IVar (Para (''InvSet'') i)) (Const true)) , (eqn (IVar (Ident ''ExGntd'')) (Const true)) ])
-(eqn (IVar (Para (''Chan3.Cmd'') j)) (Const Empty)) "
-
-definition inv_30 :: "nat \<Rightarrow> nat \<Rightarrow> formula" where [simp]:
-	"inv_30 i j \<equiv>
-		implyForm (andForm (neg (eqn (Const (index i)) (Const (index j)))) (eqn (IVar (Para (''Chan2.Cmd'') i)) (Const GntE)) )
-(eqn (IVar (Para (''Chan3.Cmd !'') j)) (Const InvAck)) "
-
-definition inv_31 :: "nat \<Rightarrow> nat \<Rightarrow> formula" where [simp]:
-	"inv_31 i j \<equiv>
-		implyForm (andForm (neg (eqn (Const (index i)) (Const (index j)))) (eqn (IVar (Para (''InvSet'') i)) (Const true)) )
-(eqn (IVar (Para (''Chan2.Cmd !'') j)) (Const GntE)) "
-
-definition inv_32 :: "nat \<Rightarrow> nat \<Rightarrow> formula" where [simp]:
-	"inv_32 i j \<equiv>
-		implyForm (andForm (neg (eqn (Const (index i)) (Const (index j)))) (eqn (IVar (Para (''Cache.State'') i)) (Const E)) )
-(eqn (IVar (Para (''InvSet'') j)) (Const false)) "
-
-definition inv_33 :: "nat \<Rightarrow> nat \<Rightarrow> formula" where [simp]:
-	"inv_33 i j \<equiv>
-		implyForm (andList [(neg (eqn (Const (index i)) (Const (index j)))), (eqn (IVar (Para (''InvSet'') i)) (Const true)) , (eqn (IVar (Ident ''ExGntd'')) (Const true)) ])
-(eqn (IVar (Para (''Chan2.Cmd'') j)) (Const Empty)) "
-
-definition inv_34 :: "nat \<Rightarrow> nat \<Rightarrow> formula" where [simp]:
-	"inv_34 i j \<equiv>
-		implyForm (andForm (neg (eqn (Const (index i)) (Const (index j)))) (eqn (IVar (Para (''Cache.State'') i)) (Const S)) )
-(eqn (IVar (Para (''Chan2.Cmd !'') j)) (Const GntE)) "
-
-definition inv_35 :: "nat \<Rightarrow> nat \<Rightarrow> formula" where [simp]:
-	"inv_35 i j \<equiv>
-		implyForm (andList [(neg (eqn (Const (index i)) (Const (index j)))), (eqn (IVar (Ident ''ExGntd'')) (Const true)) , (eqn (IVar (Para (''Chan3.Cmd'') i)) (Const InvAck)) ])
-(eqn (IVar (Para (''Chan3.Cmd'') j)) (Const Empty)) "
-
-definition inv_36 :: "nat \<Rightarrow> nat \<Rightarrow> formula" where [simp]:
-	"inv_36 i j \<equiv>
-		implyForm (andForm (neg (eqn (Const (index i)) (Const (index j)))) (eqn (IVar (Para (''Chan2.Cmd'') i)) (Const Inv)) )
-(eqn (IVar (Para (''Chan2.Cmd !'') j)) (Const GntE)) "
-
-definition inv_37 :: "nat \<Rightarrow> nat \<Rightarrow> formula" where [simp]:
-	"inv_37 i j \<equiv>
-		implyForm (andForm (neg (eqn (Const (index i)) (Const (index j)))) (eqn (IVar (Para (''Chan2.Cmd'') i)) (Const GntE)) )
-(eqn (IVar (Para (''Chan3.Cmd'') j)) (Const Empty)) "
-
-definition inv_38 :: "nat \<Rightarrow> nat \<Rightarrow> formula" where [simp]:
-	"inv_38 i j \<equiv>
-		implyForm (andForm (neg (eqn (Const (index i)) (Const (index j)))) (eqn (IVar (Para (''Cache.State'') i)) (Const E)) )
-(eqn (IVar (Para (''Chan3.Cmd'') j)) (Const Empty)) "
-
-definition inv_39 :: "nat \<Rightarrow> nat \<Rightarrow> formula" where [simp]:
-	"inv_39 i j \<equiv>
-		implyForm (andForm (neg (eqn (Const (index i)) (Const (index j)))) (eqn (IVar (Para (''Chan2.Cmd'') i)) (Const GntE)) )
-(eqn (IVar (Para (''ShrSet'') j)) (Const false)) "
-
-definition inv_40 :: "nat \<Rightarrow> nat \<Rightarrow> formula" where [simp]:
-	"inv_40 i j \<equiv>
-		implyForm (andForm (neg (eqn (Const (index i)) (Const (index j)))) (eqn (IVar (Para (''Cache.State'') i)) (Const S)) )
-(eqn (IVar (Para (''Cache.State !'') j)) (Const E)) "
-
-definition inv_41 :: "nat \<Rightarrow> nat \<Rightarrow> formula" where [simp]:
-	"inv_41 i j \<equiv>
-		implyForm (andList [(neg (eqn (Const (index i)) (Const (index j)))), (eqn (IVar (Ident ''ExGntd'')) (Const true)) , (eqn (IVar (Para (''Chan3.Cmd'') i)) (Const InvAck)) ])
-(eqn (IVar (Para (''Chan2.Cmd'') j)) (Const Empty)) "
-
-definition inv_42 :: "nat \<Rightarrow> nat \<Rightarrow> formula" where [simp]:
-	"inv_42 i j \<equiv>
-		implyForm (andList [(neg (eqn (Const (index i)) (Const (index j)))), (eqn (IVar (Para (''InvSet'') i)) (Const true)) , (eqn (IVar (Ident ''CurCmd'')) (Const ReqS)) ])
-(eqn (IVar (Para (''Chan2.Cmd !'') j)) (Const Inv)) "
-
-definition inv_43 :: "nat \<Rightarrow> nat \<Rightarrow> formula" where [simp]:
-	"inv_43 i j \<equiv>
-		implyForm (andList [(neg (eqn (Const (index i)) (Const (index j)))), (eqn (IVar (Ident ''ExGntd'')) (Const true)) , (eqn (IVar (Para (''Chan3.Cmd'') i)) (Const InvAck)) ])
-(eqn (IVar (Para (''InvSet'') j)) (Const false)) "
-
-definition inv_44 :: "nat \<Rightarrow> nat \<Rightarrow> formula" where [simp]:
-	"inv_44 i j \<equiv>
-		implyForm (andForm (neg (eqn (Const (index i)) (Const (index j)))) (eqn (IVar (Para (''Chan2.Cmd'') i)) (Const Inv)) )
-(eqn (IVar (Para (''Cache.State !'') j)) (Const E)) "
-
-definition inv_45 :: "nat \<Rightarrow> nat \<Rightarrow> formula" where [simp]:
-	"inv_45 i j \<equiv>
-		implyForm (andList [(neg (eqn (Const (index i)) (Const (index j)))), (eqn (IVar (Para (''InvSet'') i)) (Const true)) , (eqn (IVar (Ident ''ExGntd'')) (Const true)) ])
-(eqn (IVar (Para (''Chan3.Cmd !'') j)) (Const InvAck)) "
-
-definition inv_46 :: "nat \<Rightarrow> nat \<Rightarrow> formula" where [simp]:
-	"inv_46 i j \<equiv>
-		implyForm (andForm (neg (eqn (Const (index i)) (Const (index j)))) (eqn (IVar (Para (''Chan2.Cmd'') i)) (Const GntS)) )
-(eqn (IVar (Para (''Cache.State !'') j)) (Const E)) "
-
-definition inv_47 :: "nat \<Rightarrow> nat \<Rightarrow> formula" where [simp]:
-	"inv_47 i j \<equiv>
-		implyForm (andList [(neg (eqn (Const (index i)) (Const (index j)))), (eqn (IVar (Ident ''ExGntd'')) (Const true)) , (eqn (IVar (Para (''Chan3.Cmd'') i)) (Const InvAck)) ])
-(eqn (IVar (Para (''ShrSet'') j)) (Const false)) "
-
-definition inv_48 :: "nat \<Rightarrow> nat \<Rightarrow> formula" where [simp]:
-	"inv_48 i j \<equiv>
-		implyForm (andForm (neg (eqn (Const (index i)) (Const (index j)))) (eqn (IVar (Para (''Chan3.Cmd'') i)) (Const InvAck)) )
-(eqn (IVar (Para (''Chan2.Cmd !'') j)) (Const GntE)) "
-
-definition inv_49 :: "nat \<Rightarrow> nat \<Rightarrow> formula" where [simp]:
-	"inv_49 i j \<equiv>
-		implyForm (andForm (neg (eqn (Const (index i)) (Const (index j)))) (eqn (IVar (Para (''Chan2.Cmd'') i)) (Const GntS)) )
-(eqn (IVar (Para (''Chan2.Cmd !'') j)) (Const GntE)) "
-
-definition inv_50 :: "nat \<Rightarrow> nat \<Rightarrow> formula" where [simp]:
-	"inv_50 i j \<equiv>
-		implyForm (andList [(neg (eqn (Const (index i)) (Const (index j)))), (eqn (IVar (Para (''InvSet'') i)) (Const true)) , (eqn (IVar (Ident ''CurCmd'')) (Const ReqS)) ])
-(eqn (IVar (Para (''Chan3.Cmd !'') j)) (Const InvAck)) "
-
-definition inv_51 :: "nat \<Rightarrow> nat \<Rightarrow> formula" where [simp]:
-	"inv_51 i j \<equiv>
-		implyForm (andForm (neg (eqn (Const (index i)) (Const (index j)))) (eqn (IVar (Para (''Chan2.Cmd'') i)) (Const GntE)) )
-(eqn (IVar (Para (''Cache.State !'') j)) (Const S)) "
-
-definition inv_52 :: "nat \<Rightarrow> nat \<Rightarrow> formula" where [simp]:
-	"inv_52 i j \<equiv>
-		implyForm (andForm (neg (eqn (Const (index i)) (Const (index j)))) (eqn (IVar (Para (''Cache.State'') i)) (Const E)) )
-(eqn (IVar (Para (''Chan3.Cmd !'') j)) (Const InvAck)) "
-
-definition inv_53 :: "nat \<Rightarrow> nat \<Rightarrow> formula" where [simp]:
-	"inv_53 i j \<equiv>
-		implyForm (andList [(neg (eqn (Const (index i)) (Const (index j)))), (eqn (IVar (Ident ''ExGntd'')) (Const true)) , (eqn (IVar (Para (''Chan3.Cmd'') i)) (Const InvAck)) ])
-(eqn (IVar (Para (''Chan3.Cmd !'') j)) (Const InvAck)) "
-
-definition inv_54 :: "nat \<Rightarrow> nat \<Rightarrow> formula" where [simp]:
-	"inv_54 i j \<equiv>
-		implyForm (andForm (neg (eqn (Const (index i)) (Const (index j)))) (eqn (IVar (Para (''Cache.State'') i)) (Const E)) )
-(eqn (IVar (Para (''ShrSet'') j)) (Const false)) "
-
-definition inv_55 :: "nat \<Rightarrow> nat \<Rightarrow> formula" where [simp]:
-	"inv_55 i j \<equiv>
-		implyForm (andList [(neg (eqn (Const (index i)) (Const (index j)))), (eqn (IVar (Ident ''ExGntd'')) (Const true)) , (eqn (IVar (Para (''Chan3.Cmd'') i)) (Const InvAck)) ])
-(eqn (IVar (Para (''Chan2.Cmd !'') j)) (Const Inv)) "
-
-definition inv_56 :: "nat \<Rightarrow> nat \<Rightarrow> formula" where [simp]:
-	"inv_56 i j \<equiv>
-		implyForm (andForm (neg (eqn (Const (index i)) (Const (index j)))) (eqn (IVar (Para (''Cache.State'') i)) (Const E)) )
-(eqn (IVar (Para (''Chan2.Cmd !'') j)) (Const Inv)) "
-
-definition inv_57 :: "nat \<Rightarrow> nat \<Rightarrow> formula" where [simp]:
-	"inv_57 i j \<equiv>
-		implyForm (andForm (neg (eqn (Const (index i)) (Const (index j)))) (eqn (IVar (Para (''Chan2.Cmd'') i)) (Const GntE)) )
-(eqn (IVar (Para (''Cache.State'') j)) (Const I)) "
-
-definition inv_58 :: "nat \<Rightarrow> nat \<Rightarrow> formula" where [simp]:
-	"inv_58 i j \<equiv>
-		implyForm (andForm (neg (eqn (Const (index i)) (Const (index j)))) (eqn (IVar (Para (''Cache.State'') i)) (Const E)) )
-(eqn (IVar (Para (''Chan2.Cmd !'') j)) (Const GntE)) "
-
-definition inv_59 :: "nat \<Rightarrow> nat \<Rightarrow> formula" where [simp]:
-	"inv_59 i j \<equiv>
-		implyForm (andForm (neg (eqn (Const (index i)) (Const (index j)))) (eqn (IVar (Para (''Chan2.Cmd'') i)) (Const GntE)) )
-(eqn (IVar (Para (''Chan2.Cmd !'') j)) (Const GntE)) "
-
-definition inv_60 :: "nat \<Rightarrow> nat \<Rightarrow> formula" where [simp]:
-	"inv_60 i j \<equiv>
-		implyForm (andList [(neg (eqn (Const (index i)) (Const (index j)))), (eqn (IVar (Para (''InvSet'') i)) (Const true)) , (eqn (IVar (Ident ''ExGntd'')) (Const true)) ])
-(eqn (IVar (Para (''Chan2.Cmd !'') j)) (Const Inv)) "
-
-definition inv_61 :: "nat \<Rightarrow> nat \<Rightarrow> formula" where [simp]:
-	"inv_61 i j \<equiv>
-		implyForm (andForm (neg (eqn (Const (index i)) (Const (index j)))) (eqn (IVar (Para (''Chan2.Cmd'') i)) (Const GntE)) )
-(eqn (IVar (Para (''Chan2.Cmd !'') j)) (Const Inv)) "
-
-definition inv_62 :: "nat \<Rightarrow> nat \<Rightarrow> formula" where [simp]:
-	"inv_62 i j \<equiv>
-		implyForm (andForm (neg (eqn (Const (index i)) (Const (index j)))) (eqn (IVar (Para (''Cache.State'') i)) (Const E)) )
-(eqn (IVar (Para (''Cache.State !'') j)) (Const E)) "
 
 subsection{*Definitions of each abstracted rule*}
 
 definition  NC::"nat " where [simp]: "NC==1"
 
-definition n_SendGntE3_i::"nat \<Rightarrow> nat \<Rightarrow> rule" where [simp]:
-"n_SendGntE3_i  i N\<equiv>
-let g = (andList [(eqn (IVar (Ident ''CurCmd'')) (Const ReqE)) , (eqn (IVar (Ident ''CurPtr'')) (IVar (Ident '' Other''))) , (eqn (IVar (Ident ''ExGntd'')) (Const false)) , (forallForm (down N) (\<lambda>j. (eqn (IVar (Para (''ShrSet'') i)) (Const false)) ))])in
-let s = (parallelList [(assign ((Ident ''ExGntd''), (Const true ))), (assign ((Ident ''	CurCmd''), (Const Empty)))]) in
-guard g s"
+definition n_SendGntE3_abs::"nat \<Rightarrow> nat \<Rightarrow> rule" where [simp]:
+"n_SendGntE3_abs  i M\<equiv>
+(IVar (Ident ''CurCmd''))  =\<^sub>f (Const ReqE)  \<and>\<^sub>f
+(IVar (Ident ''CurPtr''))  =\<^sub>f (Const (index (M+1)))  \<and>\<^sub>f
+(IVar (Ident ''ExGntd''))  =\<^sub>f (Const false)  \<and>\<^sub>f
+(\<forall>\<^sub>fj. (IVar (Para (''ShrSet\'') j)) =\<^sub>f  (Const false) )) M
 
-definition n_SendGntS4_i::"nat \<Rightarrow> rule" where [simp]:
-"n_SendGntS4_i  i\<equiv>
-let g = (andList [(eqn (IVar (Ident ''CurCmd'')) (Const ReqS)) , (eqn (IVar (Ident ''CurPtr'')) (IVar (Ident '' Other''))) , (eqn (IVar (Ident ''ExGntd'')) (Const false)) ])in
-let s = (parallelList [(assign ((Ident ''CurCmd''), (Const Empty)))]) in
-guard g s"
+   \<triangleright>
+(assign ((Ident ''ExGntd''), (Const true )))||
+(assign ((Ident ''	CurCmd''), (Const Empty)))"
 
-definition n_RecvInvAck5_i::"nat \<Rightarrow> nat \<Rightarrow> rule" where [simp]:
-"n_RecvInvAck5_i  i N\<equiv>
-let g = (andList [(eqn (IVar (Ident ''CurCmd !'')) (Const Empty)) , (eqn (IVar (Ident ''ExGntd'')) (Const true)) , (forallForm (down N) (\<lambda>j. (eqn (IVar (Para (''InvSet'') i)) (Const false)) )), (eqn (IVar (Para (''ShrSet'') i)) (Const false)) , (eqn (IVar (Para (''Chan3.Cmd'') i)) (Const Empty)) , (eqn (IVar (Para (''Chan2.Cmd !'') i)) (Const Inv)) , (eqn (IVar (Para (''Chan3.Cmd !'') i)) (Const InvAck)) , (eqn (IVar (Para (''Chan2.Cmd'') i)) (Const Empty)) , (eqn (IVar (Para (''Cache.State !'') i)) (Const E)) , (eqn (IVar (Para (''Cache.State'') i)) (Const I)) , (eqn (IVar (Para (''Chan2.Cmd !'') i)) (Const GntE)) ])in
-let s = (parallelList [(assign ((Ident ''ExGntd''), (Const false ))), (assign ((Ident ''	MemData''), (IVar (Ident ''AuxData''))))]) in
-guard g s"
+definition n_SendGntS4_abs::"nat \<Rightarrow> rule" where [simp]:
+"n_SendGntS4_abs  i\<equiv>
+(IVar (Ident ''CurCmd''))  =\<^sub>f (Const ReqS)  \<and>\<^sub>f
+(IVar (Ident ''CurPtr''))  =\<^sub>f (Const (index (M+1)))  \<and>\<^sub>f
+(IVar (Ident ''ExGntd''))  =\<^sub>f (Const false) 
 
-definition n_RecvReqE11_i::"nat \<Rightarrow> nat \<Rightarrow> rule" where [simp]:
-"n_RecvReqE11_i  i N\<equiv>
-let g = (eqn (IVar (Ident ''CurCmd'')) (Const Empty)) in
-let s = (parallelList [(assign ((Ident ''CurCmd''), (Const ReqE ))), (assign ((Ident ''	CurPtr''), (IVar (Ident '' Other'')))), (parallelList (map (\<lambda>j. (assign (Para (''		InvSet'') i, (IVar (Para (''ShrSet'') i))))) (down N)))]) in
-guard g s"
+   \<triangleright>
+(assign ((Ident ''CurCmd''), (Const Empty)))"
 
-definition n_RecvReqS12_i::"nat \<Rightarrow> nat \<Rightarrow> rule" where [simp]:
-"n_RecvReqS12_i  i N\<equiv>
-let g = (eqn (IVar (Ident ''CurCmd'')) (Const Empty)) in
-let s = (parallelList [(assign ((Ident ''CurCmd''), (Const ReqS ))), (assign ((Ident ''	CurPtr''), (IVar (Ident '' Other'')))), (parallelList (map (\<lambda>j. (assign (Para (''		InvSet'') i, (IVar (Para (''ShrSet'') i))))) (down N)))]) in
-guard g s"
+definition n_RecvInvAck5_abs::"nat \<Rightarrow> nat \<Rightarrow> rule" where [simp]:
+"n_RecvInvAck5_abs  i M\<equiv>
+\<not>\<^sub>f (IVar (Ident ''CurCmd'')) =\<^sub>f  (Const Empty)  \<and>\<^sub>f
+(IVar (Ident ''ExGntd''))  =\<^sub>f (Const true)  \<and>\<^sub>f
+(\<forall>\<^sub>fj. (IVar (Para (''InvSet\'') j)) =\<^sub>f  (Const false) )) M \<and>\<^sub>f
+(IVar (Para (''ShrSet\'') j)) =\<^sub>f  (Const false)  \<and>\<^sub>f
+(IVar (Para (''Chan3\.Cmd'') j)) =\<^sub>f  (Const Empty)  \<and>\<^sub>f
+\<not>\<^sub>f (IVar (Para (''Chan2\.Cmd'') j)) =\<^sub>f  (Const Inv)  \<and>\<^sub>f
+\<not>\<^sub>f (IVar (Para (''Chan3\.Cmd'') j)) =\<^sub>f  (Const InvAck)  \<and>\<^sub>f
+(IVar (Para (''Chan2\.Cmd'') j)) =\<^sub>f  (Const Empty)  \<and>\<^sub>f
+\<not>\<^sub>f (IVar (Para (''Cache\.State'') j)) =\<^sub>f  (Const E)  \<and>\<^sub>f
+(IVar (Para (''Cache\.State'') j)) =\<^sub>f  (Const I)  \<and>\<^sub>f
+\<not>\<^sub>f (IVar (Para (''Chan2\.Cmd'') j)) =\<^sub>f  (Const GntE) 
 
-definition n_Store16_i::"nat \<Rightarrow> nat \<Rightarrow> rule" where [simp]:
-"n_Store16_i  i N\<equiv>
-let g = (andList [(forallForm (down N) (\<lambda>j. (eqn (IVar (Para (''InvSet'') i)) (Const false)) )), (eqn (IVar (Para (''ShrSet'') i)) (Const false)) , (eqn (IVar (Para (''Chan3.Cmd'') i)) (Const Empty)) , (eqn (IVar (Para (''Chan2.Cmd !'') i)) (Const Inv)) , (eqn (IVar (Para (''Chan2.Cmd !'') i)) (Const GntS)) , (eqn (IVar (Para (''Chan3.Cmd !'') i)) (Const InvAck)) , (eqn (IVar (Para (''Cache.State !'') i)) (Const S)) , (eqn (IVar (Para (''Chan2.Cmd'') i)) (Const Empty)) , (eqn (IVar (Para (''Cache.State !'') i)) (Const E)) , (eqn (IVar (Para (''Cache.State'') i)) (Const I)) , (eqn (IVar (Ident ''ExGntd'')) (Const true)) , (eqn (IVar (Para (''Chan2.Cmd !'') i)) (Const GntE)) ])in
-let s = (parallelList [(assign ((Ident ''AuxData''), (IVar (Ident ''['DATA_1']''))))]) in
-guard g s"
+   \<triangleright>
+(assign ((Ident ''ExGntd''), (Const false )))||
+(assign ((Ident ''	MemData''), (IVar (Ident ''AuxData''))))"
+
+definition n_RecvReqE11_abs::"nat \<Rightarrow> nat \<Rightarrow> rule" where [simp]:
+"n_RecvReqE11_abs  i M\<equiv>
+(IVar (Ident ''CurCmd''))  =\<^sub>f (Const Empty) 
+   \<triangleright>
+(assign ((Ident ''CurCmd''), (Const ReqE )))||
+(assign ((Ident ''	CurPtr''), (IVar (Ident '' Other''))))||
+(parallelList (map (\<lambda>j. (assign (Para (''		InvSet\'') j, (IVar (Para (''ShrSet\'') j))))) (down N)))"
+
+definition n_RecvReqS12_abs::"nat \<Rightarrow> nat \<Rightarrow> rule" where [simp]:
+"n_RecvReqS12_abs  i M\<equiv>
+(IVar (Ident ''CurCmd''))  =\<^sub>f (Const Empty) 
+   \<triangleright>
+(assign ((Ident ''CurCmd''), (Const ReqS )))||
+(assign ((Ident ''	CurPtr''), (IVar (Ident '' Other''))))||
+(parallelList (map (\<lambda>j. (assign (Para (''		InvSet\'') j, (IVar (Para (''ShrSet\'') j))))) (down N)))"
+
+definition n_Store16_abs::"nat \<Rightarrow> nat \<Rightarrow> rule" where [simp]:
+"n_Store16_abs  i M\<equiv>
+(\<forall>\<^sub>fj. (IVar (Para (''InvSet\'') j)) =\<^sub>f  (Const false) )) M \<and>\<^sub>f
+(IVar (Para (''ShrSet\'') j)) =\<^sub>f  (Const false)  \<and>\<^sub>f
+(IVar (Para (''Chan3\.Cmd'') j)) =\<^sub>f  (Const Empty)  \<and>\<^sub>f
+\<not>\<^sub>f (IVar (Para (''Chan2\.Cmd'') j)) =\<^sub>f  (Const Inv)  \<and>\<^sub>f
+\<not>\<^sub>f (IVar (Para (''Chan2\.Cmd'') j)) =\<^sub>f  (Const GntS)  \<and>\<^sub>f
+\<not>\<^sub>f (IVar (Para (''Chan3\.Cmd'') j)) =\<^sub>f  (Const InvAck)  \<and>\<^sub>f
+\<not>\<^sub>f (IVar (Para (''Cache\.State'') j)) =\<^sub>f  (Const S)  \<and>\<^sub>f
+(IVar (Para (''Chan2\.Cmd'') j)) =\<^sub>f  (Const Empty)  \<and>\<^sub>f
+\<not>\<^sub>f (IVar (Para (''Cache\.State'') j)) =\<^sub>f  (Const E)  \<and>\<^sub>f
+(IVar (Para (''Cache\.State'') j)) =\<^sub>f  (Const I)  \<and>\<^sub>f
+(IVar (Ident ''ExGntd''))  =\<^sub>f (Const true)  \<and>\<^sub>f
+\<not>\<^sub>f (IVar (Para (''Chan2\.Cmd'') j)) =\<^sub>f  (Const GntE) 
+
+   \<triangleright>
+(assign ((Ident ''AuxData''), (IVar (Ident ''['DATA_1']''))))"
 
 
 
